remove deprecated weak_subst proof, delete old fun typing files, rename and rearrange subst lemmatas

IMLTT/untyped/proofs/Mixture.lean
@@ -15,11 +15,12 @@ open Lean.Meta
 open Lean.Elab.Tactic
 open Lean.TSyntax
 
--- use macros
+-- macros for easier usage of de bruijn abstractions
+-- FIXME: extraxt macros to other file
 
 macro "context_info_nat_relations" : tactic =>
   `(tactic|
-      (first -- FIXME: find way to do all lemmatas for all available contexts (repeat' not possible)
+      (first
         | have := by
             apply gen_ctx_leq
             assumption
@@ -100,10 +101,58 @@ macro "weakening_var_weak" : tactic =>
       cases' i with i'
      ))
 
+macro "conversion_var_sub_symm" : tactic =>
+  `(tactic|
+    (
+      apply Eq.symm
+      apply conversion_var_substitute
+      intro x
+      cases' x with i hFin
+      cases' i with i'
+     ))
+
 macro "conversion_var_sub" : tactic =>
   `(tactic|
     (
       apply conversion_var_substitute
+      intro x
+      cases' x with i hFin
+      cases' i with i'
+     ))
+
+macro "substitution_var_substitute_id" : tactic =>
+  `(tactic|
+    (
+      apply substitution_var_substitute_id
+      intro x
+      cases' x with i hFin
+      cases' i with i'
+     ))
+
+macro "substitution_var_substitute_id_symm" : tactic =>
+  `(tactic|
+    (
+      apply Eq.symm
+      apply substitution_var_substitute_id
+      intro x
+      cases' x with i hFin
+      cases' i with i'
+     ))
+
+macro "weakening_var_weaken_id" : tactic =>
+  `(tactic|
+    (
+      apply weakening_var_weaken_id
+      intro x
+      cases' x with i hFin
+      cases' i with i'
+     ))
+
+macro "weakening_var_weaken_id_symm" : tactic =>
+  `(tactic|
+    (
+      apply Eq.symm
+      apply weakening_var_weaken_id
       intro x
       cases' x with i hFin
       cases' i with i'
@@ -119,8 +168,8 @@ macro "substitution_split" : tactic =>
         cases heq
      ))
 
-
-def cases (id : FVarId) : TacticM Unit := -- XXX: aus interactive theorem proving repo
+-- meta cases tactic
+def cases (id : FVarId) : TacticM Unit := -- XXX: from interactive theorem proving repo
   do
     liftMetaTactic (fun goal ↦
       do
@@ -132,14 +181,15 @@ def cases (id : FVarId) : TacticM Unit := -- XXX: aus interactive theorem provin
 partial def useCases : TacticM Unit :=
   withMainContext
     (do
-       let lctx ← getLCtx
-       for ldecl in lctx do
-         if ! LocalDecl.isImplementationDetail ldecl then
-           if Expr.isAppOfArity (LocalDecl.type ldecl) ``Eq 3
-            then -- FIXME: how to abort, if dependent elimination breaks this? e.g. on cases heqΓ
-                 -- use simple try block?
+      let lctx ← getLCtx
+      for ldecl in lctx do
+        if ! LocalDecl.isImplementationDetail ldecl then
+          if Expr.isAppOfArity (LocalDecl.type ldecl) ``Eq 3 then
+            try
               cases (LocalDecl.fvarId ldecl)
-              -- return
+            catch _ =>
+              logInfo m!"error on case: {ldecl.type}, stopping here"
+              return
     )
 
 elab "use_cases" : tactic =>
@@ -160,6 +210,15 @@ macro "substitution_step" : tactic =>
         try substitution_var_sub
         try weakening_var_weak
         try conversion_var_sub
+        try conversion_var_sub_symm
+        -- FIXME: when t = t⌈σ⌉ or with ρ,
+        --        problems when either side of eq is placeholder
+        --        divide into two major macros, one with and one without?
+        --
+        -- try substitution_var_substitute_id
+        -- try substitution_var_substitute_id_symm
+        -- try weakening_var_weaken_id
+        -- try weakening_var_weaken_id_symm
         try substitution_from_composition
         try simp []
         try split_and_cases
@@ -168,27 +227,35 @@ macro "substitution_step" : tactic =>
         try any_goals rfl
         ))
 
-macro "substitution_norm" : tactic => -- FIXME: still infinite, because haves, needs if_goal_unchanged
+macro "substitution_norm" : tactic =>
   `(tactic|
       (
         repeat' (fail_if_no_progress substitution_step)
         ))
 
 
+-- FIXME:
+-- - change all theorems to not use ⌈-⌉₀ anymore? or add simp ones
+-- - name changes -> also in helper files
 
-
--- FIXME: change al theorems to not use ⌈-⌉₀ anymore? or add simp ones
-
-theorem weak_sub_zero :
+theorem substitution_zero_weak :
     t⌈a⌉₀⌊ρ⌋ = t⌊⇑ₚρ⌋⌈a⌊ρ⌋⌉₀ :=
   by
     substitution_norm
 
-theorem weak_sub_shift :
-    t⌈(ₛ↑ₚidₚ)⋄ a⌉⌊⇑ₚρ⌋ = t⌊⇑ₚρ⌋⌈(ₛ↑ₚidₚ)⋄ (a⌊⇑ₚρ⌋)⌉ :=
+@[simp]
+theorem substitution_zero_weak_simp :
+    t⌊⇑ₚρ⌋⌈(ₛidₚ)⋄ (a⌊ρ⌋)⌉ = t⌈(ₛidₚ)⋄ a⌉⌊ρ⌋ :=
   by
     substitution_norm
 
+@[simp]
+theorem substitution_lift_weak_subst :
+    t⌊⇑ₚρ⌋⌈(ₛ↑ₚidₚ)⋄ (a⌊⇑ₚρ⌋)⌉ = t⌈(ₛ↑ₚidₚ)⋄ a⌉⌊⇑ₚρ⌋ :=
+  by
+    substitution_norm
+
+@[simp]
 theorem substitution_var_single_comp :
     v(x)⌈(ₛidₚ)⋄ a ₛ∘ₛ⇑ₛσ⌉ = v(x)⌈σ⋄ a⌉ :=
   by
@@ -254,31 +321,26 @@ theorem substitution_extend :
   by
     substitution_norm
 
+@[simp]
 theorem substitution_extend_lift :
-    t⌈⇑ₛσ⌉⌊⇑ₚρ⌋⌈a⌉₀ = t⌈ρ ₚ∘ₛσ⋄ a⌉ :=
+    t⌈⇑ₛσ⌉⌊⇑ₚρ⌋⌈(ₛidₚ)⋄ a⌉ = t⌈ρ ₚ∘ₛσ⋄ a⌉ :=
   by
     substitution_norm
 
 @[simp]
+theorem substitution_zero_lift_simp :
+    t⌈⇑ₛσ⌉⌈(ₛidₚ)⋄ (a⌈σ⌉)⌉ = t⌈(ₛidₚ)⋄ a⌉⌈σ⌉ :=
+  by
+    substitution_norm
+
 theorem substitution_zero_lift :
     t⌈a⌉₀⌈σ⌉ = t⌈⇑ₛσ⌉⌈a⌈σ⌉⌉₀ :=
   by
     substitution_norm
 
 @[simp]
-theorem idWkLiftSubstLemma :
-    t⌈⇑ₛσ⌉⌊⇑ₚ↑ₚidₚ⌋⌈v(0)⌉₀ = t⌈⇑ₛσ⌉ :=
-  by
-    substitution_norm
-
-theorem singleSubstLift :
-    t⌈(ₛ↑ₚidₚ)⋄ a⌉⌈⇑ₛσ⌉ = t⌈⇑ₛσ⌉⌈(ₛ↑ₚidₚ)⋄ (a⌈⇑ₛσ⌉)⌉ :=
-  by
-    substitution_norm
-
--- own
-theorem lift_single_subst_tt :
-   A⌊⇑ₚweaken_from n l⌋⌈⋆⌉₀ = A⌈⋆⌉₀⌊weaken_from n l⌋ :=
+theorem substitution_shift_lift_zero :
+    t⌈⇑ₛσ⌉⌊⇑ₚ↑ₚidₚ⌋⌈(ₛidₚ)⋄ v(0)⌉ = t⌈⇑ₛσ⌉ :=
   by
     substitution_norm
 
@@ -293,18 +355,14 @@ theorem substitution_shift_substitute_zero_simp :
   by
     substitution_norm
 
-theorem substitution_twice_zero {n : Nat} {T : Tm (n + 2)} {b : Tm (n)} {a : Tm (n)} :
-    T⌈(ₛidₚ)⋄ a⋄ b⌉ = T⌈b⌊↑ₚidₚ⌋⌉₀⌈a⌉₀ :=
-  by
-    substitution_norm
-
+@[simp]
 theorem substitution_separate {n m : Nat} {t : Tm (n + 1)} {s : Tm m} {σ : Subst m n} :
-    t⌈σ⋄ s⌉ = t⌈⇑ₛσ⌉⌈s⌉₀ :=
+    t⌈⇑ₛσ⌉⌈(ₛidₚ)⋄ s⌉ = t⌈σ⋄ s⌉ :=
   by
     substitution_norm
 
 @[simp]
-theorem substitution_weak_id : -- TODO: can be generalized to v(i)
+theorem substitution_weak_id_shift :
     B⌈(ₛ↑ₚ↑ₚidₚ)⋄ v(1)⌉ = B⌊↑ₚidₚ⌋ :=
   by
     rw (config := {occs := .pos [2]}) [←substitution_id (t := B)]
@@ -372,3 +430,14 @@ theorem weak_substitution_eq_weakening_substitution_gen_context {l n : Nat} {s :
       apply And.intro
       · rw [ih]
       · rw [weak_substitution_eq_weakening_substitution]
+
+-- theorem test_id_thing_lol :
+--     B⌈⇑ₛ(ₛidₚ)⌉ = B :=
+--   by
+--     substitution_norm
+--
+-- theorem test_id_complicated_thing_lol :
+--     B⌊⇑ₚ↑ₚidₚ⌋⌈A⌊↑ₚidₚ⌋.indSigma (B⌊1ₙ⇑ₚ(↑ₚidₚ)⌋) (A⌊↑ₚidₚ⌋⌊↑ₚidₚ⌋) (v(0)⌊↑ₚidₚ⌋) v(0)⌉₀⌈a&b⌉₀
+--     = B⌈A.indSigma B (A⌊↑ₚidₚ⌋) v(1) (a&b)⌉₀ :=
+--   by
+--     substitution_norm
