IMLTT.lean
@@ -1,2 +1,4 @@
 import «IMLTT».Basic
 import IMLTT.typed.proofs.boundary.BoundaryTypesTerms
+import IMLTT.typed.SigmaProjections
+import IMLTT.typed.PropositionalEquality
