IMLTT/typed/proofs/admissable/FunctionalityTyping.lean
@@ -390,11 +390,6 @@ theorem functionality_typing_general_term {n l : Nat} {Γ : Ctx l} {Δ : CtxGen 
     · apply hsS'
     · apply hT
 
-    -- (∀ {n l : Nat} {Γ : Ctx l} {Δ : CtxGen (l + 1) (n + 1)} {T : Tm (n + 1)} {s s' S : Tm l},
-    --   (Γ ⊢ s ≡ s' ∶ S) → (Γ ⊢ s ∶ S) → (Γ ⊢ s' ∶ S)
-    --   → (Γ ⬝ S ⊗ Δ ⊢ T type)
-    --   → (Γ ⊗ ⌈s⌉(Δ w/Nat.le_refl l)) ⊢ (T⌈s/ₙ (Nat.le_of_succ_le_succ (gen_ctx_leq Δ))⌉) ≡ (T⌈s'/ₙ (Nat.le_of_succ_le_succ (gen_ctx_leq Δ))⌉) type
-    -- ) ∧
 theorem functionality_typing_term {l : Nat} {Γ : Ctx l} {s s' S : Tm l} {t T : Tm (l + 1)} :
       (Γ ⬝ S ⊢ t ∶ T)
       → (Γ ⊢ s ≡ s' ∶ S) → (Γ ⊢ s ∶ S) → (Γ ⊢ s' ∶ S)
