IMLTT/typed/proofs/admissable/Substitution/Helpers.lean
@@ -10,37 +10,34 @@ theorem subst_subst_sigma_c :
     c⌈(ₛidₚ)⋄ a⋄ b⌉⌈σ⌉
     = c⌈lift_subst_n 2 σ⌉⌈(ₛidₚ)⋄ (a⌈σ⌉)⋄ (b⌈σ⌉)⌉ :=
   by
-    substitution_step
+    substitution_norm
 
 theorem subst_subst_sigma_C :
     C⌈⇑ₛσ⌉⌈(ₛ↑ₚ↑ₚidₚ)⋄ v(1)&v(0)⌉ =
     C⌈(ₛ↑ₚ↑ₚidₚ)⋄ v(1)&v(0)⌉⌈⇑ₛ⇑ₛσ⌉ :=
   by
-    substitution_step
-    substitution_step
+    substitution_norm
 
 theorem subst_subst_iden_refl :
     B⌈3ₙ⇑ₛ(σ)⌉⌈(ₛidₚ)⋄ v(0)⋄ (A⌊↑ₚidₚ⌋⌈⇑ₛ(σ)⌉.refl v(0))⌉
     = B⌈(ₛidₚ)⋄ v(0)⋄ (A⌊↑ₚidₚ⌋.refl v(0))⌉⌈⇑ₛ(σ)⌉ :=
   by
-    substitution_step
+    substitution_norm
 
 theorem subst_subst_iden_elim :
     B⌈(ₛidₚ)⋄ a⋄ b⋄ c⌉⌈σ⌉
     = B⌈lift_subst_n 3 σ⌉⌈(ₛidₚ)⋄ (a⌈σ⌉)⋄ (b⌈σ⌉)⋄ (c⌈σ⌉)⌉ :=
   by
-    substitution_step
+    substitution_norm
 
 theorem helper_subst_iden_propagate_subst :
     (v(1) ≃[A⌊↑ₚ↑ₚidₚ⌋] v(0))⌈⇑ₛ⇑ₛσ⌉
     = v(1) ≃[A⌊↑ₚ↑ₚidₚ⌋⌈⇑ₛ⇑ₛσ⌉] v(0) :=
   by
-    substitution_step
-    substitution_step
+    substitution_norm
 
 theorem helper_subst_nat_elim {s : Tm l} {A : Tm (n + 2)} :
     A⌈(ₛ↑ₚidₚ)⋄ 𝓈(v(0))⌉⌊↑ₚidₚ⌋⌈⇑ₛ⇑ₛ(s/ₙhleq)⌉
     = A⌈⇑ₛ(s/ₙhleq)⌉⌈(ₛ↑ₚidₚ)⋄ 𝓈(v(0))⌉⌊↑ₚidₚ⌋ :=
   by
-    substitution_step
-    substitution_step
+    substitution_norm
