IMLTT/typed/proofs/admissable/Weakening/Helpers.lean
@@ -13,51 +13,37 @@ import IMLTT.typed.proofs.boundary.BoundaryIsCtx
 theorem shift_weaken_from {hl : l ≤ n} :
     A⌊↑ₚidₚ⌋⌊weaken_from (n + 1) l⌋ = A⌊weaken_from n l⌋⌊↑ₚidₚ⌋ :=
   by
-    substitution_nat_relation_lemmatas
-    substitution_step
+    substitution_norm
 
 theorem weak_subst_sigma_C {leq : l ≤ n}:
     C⌊weaken_from (n + 1) l⌋⌈(ₛ↑ₚ↑ₚidₚ)⋄ v(1)&v(0)⌉ =
     C⌈(ₛ↑ₚ↑ₚidₚ)⋄ v(1)&v(0)⌉⌊weaken_from (n + 1 + 1) l⌋ :=
   by
-    substitution_nat_relation_lemmatas
-    substitution_step
-    substitution_step
+    substitution_norm
 
 theorem weak_subst_sigma_c :
     c⌈(ₛidₚ)⋄ a⋄ b⌉⌊ρ⌋
     = c⌊2ₙ⇑ₚρ⌋⌈(ₛidₚ)⋄ (a⌊ρ⌋)⋄ (b⌊ρ⌋)⌉ :=
   by
-    substitution_step
-    aesop
+    substitution_norm
 
 theorem weak_subst_iden_elim :
     B⌈(ₛidₚ)⋄ a⋄ b⋄ c⌉⌊ρ⌋
     = B⌊lift_weak_n 3 ρ⌋⌈(ₛidₚ)⋄ (a⌊ρ⌋)⋄ (b⌊ρ⌋)⋄ (c⌊ρ⌋)⌉ :=
   by
-    substitution_step
-    aesop
+    substitution_norm
 
 theorem helper_weak_iden_propagate_weak {leq : l ≤ n} :
     (v(1) ≃[A⌊↑ₚ↑ₚidₚ⌋] v(0))⌊weaken_from (n + 1 + 1) l⌋
     = v(1) ≃[A⌊↑ₚ↑ₚidₚ⌋⌊weaken_from (n + 1 + 1) l⌋] v(0) :=
   by
-    substitution_nat_relation_lemmatas
-    substitution_step
-    substitution_step
+    substitution_norm
 
 theorem helper_weak_refl_propagate_weak {leq : l ≤ n} :
     B⌊⇑ₚ⇑ₚ↑₁n + 1↬l⌋⌈(ₛidₚ)⋄ v(0)⋄ (A⌊↑₁n↬l⌋⌊↑ₚidₚ⌋.refl v(0))⌉
     = B⌈(ₛidₚ)⋄ v(0)⋄ (A⌊↑ₚidₚ⌋.refl v(0))⌉⌊↑₁n + 1↬l⌋ :=
   by
-    substitution_nat_relation_lemmatas
-    substitution_step
-
-theorem tleq {l : Nat} :
-    l + 1 ≤ 0 -> False :=
-  by
-    intro hLeq
-    omega
+    substitution_norm
 
 theorem helper_weak_1 :
     l ≤ x → x + 1 ≤ l → False :=
@@ -69,5 +55,4 @@ theorem helper_weak_nat_succ {leq : l ≤ n} :
     A⌈(ₛ↑ₚidₚ)⋄ 𝓈(v(0))⌉⌊↑ₚidₚ⌋⌊weaken_from (n + 1 + 1) l⌋
     = A⌊1ₙ⇑ₚweaken_from n l⌋⌈(ₛ↑ₚidₚ)⋄ 𝓈(v(0))⌉⌊↑ₚidₚ⌋ :=
   by
-    substitution_step
-    substitution_step
+    substitution_norm
